Foundation/Modal/ModalCompanion/Standard/KC.lean
@@ -1,184 +1,80 @@
 module
 
-public import Foundation.Modal.ModalCompanion.Standard.Int
+public import Foundation.Logic.Embedding
+public import Foundation.Modal.Boxdot.GL_Grz
 public import Foundation.Modal.Kripke.Logic.GrzPoint2
--- public import Foundation.Propositional.Kripke.Logic.KC
+public import Foundation.Modal.ModalCompanion.Standard.Basic
+public import Foundation.Propositional.Kripke.Hilbert.KC
 
 @[expose] public section
 
-namespace LO.Propositional
-
-def Substitution.toModal (s : Propositional.Substitution α) : Modal.Substitution (α) := λ x => (s x).toModalFormula
-instance : Coe (Propositional.Substitution α) (Modal.Substitution α) := ⟨Substitution.toModal⟩
-
-end LO.Propositional
-
-
-namespace LO.Modal
+namespace LO
 
 open LO.Entailment LO.Entailment.FiniteContext LO.Modal.Entailment
 open Propositional
-open Propositional.Formula (atom gödelTranslate)
+open Propositional.Formula (gödelTranslate)
 open Propositional.Logic (smallestMC largestMC)
 open Modal
 open Modal.Kripke
-open Modal.Formula.Kripke
+
 
 namespace S4Point2
 
-open Formula.Kripke in
-lemma gödelTranslated_axiomWLEM : Modal.S4Point2 ⊢ □(∼φᵍ) ⋎ □(∼□(∼φᵍ)) := by
-  suffices Modal.S4Point2 ⊢ □(∼(□φᵍ)) ⋎ □(∼□(∼□(φᵍ))) by
-    apply A!_replace this;
-    . apply axiomK'!;
-      apply nec!;
-      apply contra!;
-      exact gödelTranslated_axiomTc;
-    . apply axiomK'!;
-      apply nec!;
-      apply contra!;
-      apply axiomK'!;
-      apply nec!;
-      apply contra!;
-      exact axiomT!
+@[simp, grind .]
+lemma gödelTranslated_axiomWLEM : Modal.S4Point2 ⊢ (Axioms.WLEM φ)ᵍ := by
   apply Complete.complete (𝓜 := FrameClass.S4Point2);
   rintro F hF V x;
   replace hF := Set.mem_setOf_eq.mp hF;
 
-  apply Formula.Kripke.Satisfies.or_def.mpr;
+  apply Modal.Formula.Kripke.Satisfies.or_def.mpr;
   by_contra! hC;
   rcases hC with ⟨h₁, h₂⟩;
 
-  replace h₁ := Formula.Kripke.Satisfies.dia_def.mp h₁;
+  replace h₁ := Modal.Formula.Kripke.Satisfies.dia_def.mp h₁;
   obtain ⟨y, Rxy, h₁⟩ := h₁;
 
-  replace h₂ := Formula.Kripke.Satisfies.dia_def.mp h₂;
+  replace h₂ := Modal.Formula.Kripke.Satisfies.dia_def.mp h₂;
   obtain ⟨z, Rxz, h₂⟩ := h₂;
 
   obtain ⟨u, Ryu, Rzu⟩ := F.ps_convergent Rxy Rxz;
-
-  have := Formula.Kripke.Satisfies.box_def.not.mp $ h₂ u Rzu;
-  push_neg at this;
-  obtain ⟨v, Ruv, h⟩ := this;
-
-  have := h₁ v $ IsTrans.trans _ _ _ Ryu Ruv
-  contradiction;
-
-instance : Entailment.HasAxiomPoint2 Propositional.KC.smallestMC where
-  Point2 φ := by
-    constructor;
-    apply Modal.Logic.iff_provable.mp;
-    apply Modal.Logic.subst (L := Propositional.KC.smallestMC) (φ := Modal.Axioms.Point2 (.atom 0)) (s := λ a => φ);
-    have : Propositional.KC.smallestMC ⊢ □(∼□(.atom 0)) ⋎ □(∼□(∼□(.atom 0))) := by
-      apply Logic.sumNormal.mem₂!;
-      use Axioms.WLEM (.atom 0);
-      constructor;
-      . apply Propositional.Logic.iff_provable.mp;
-        simp;
-      . tauto;
-    apply ?_ ⨀ this;
-    apply Entailment.WeakerThan.pbl (𝓢 := Modal.S4);
-    apply Complete.complete (𝓜 := FrameClass.S4);
-    rintro F ⟨_, _⟩ V x h₁ h₂ y Rxy;
-    replace h₁ := Satisfies.or_def.mp h₁;
-    replace h₂ := Satisfies.dia_def.mp h₂;
-    obtain ⟨z, Rxz, h₂⟩ := h₂;
-
-    rcases h₁ with (h₁ | h₁);
-    . have := h₁ z Rxz;
-      contradiction;
-    . have := Satisfies.box_def.not.mp $ Satisfies.not_def.mp $ h₁ y Rxy
-      push_neg at this;
-      obtain ⟨u, Ryu, h⟩ := this;
-      apply Satisfies.dia_def.mpr;
-      use u;
-      constructor;
-      . assumption;
-      . apply Satisfies.negneg_def.mp h u
-        apply Std.Refl.refl;
-
-instance : Modal.S4Point2 ≊ Propositional.KC.smallestMC := by
-  apply Logic.equiv_of_provable;
-  intro φ;
-  constructor;
-  . intro hφ;
-    induction hφ using Modal.Hilbert.Normal.rec! with
-    | axm s h =>
-      rcases h with (rfl | rfl | rfl | rfl) <;> simp;
-    | mdp ihφψ ihφ => exact ihφψ ⨀ ihφ;
-    | nec ihφ => exact nec! ihφ;
-    | _ => simp;
-  . intro hφ;
-    induction hφ using Logic.sumNormal.rec! with
-    | mem₁ h => apply WeakerThan.pbl h;
-    | mdp ihφψ ihψ => exact ihφψ ⨀ ihψ;
-    | nec ihφ => exact nec! ihφ;
-    | subst ihφ => apply Logic.subst _ ihφ;
-    | mem₂ h =>
-      rcases h with ⟨φ, hφ, rfl⟩;
-      apply provable_gödelTranslated_of_provable ?_ (Propositional.Logic.iff_provable.mpr hφ);
-      rintro _ ⟨_, (rfl | rfl), ⟨s, rfl⟩⟩;
-      . simp;
-      . exact S4Point2.gödelTranslated_axiomWLEM;
-
-lemma eq_smallestMC_of_KC : Modal.S4Point2 = Propositional.KC.smallestMC := Logic.eq_of_equiv
-
-instance : Sound Propositional.KC.smallestMC FrameClass.S4Point2 := Kripke.sound_frameClass_of_equiv Modal.S4Point2 Propositional.KC.smallestMC
-
-instance modalCompanion_KC_S4Point2 : ModalCompanion Propositional.KC Modal.S4Point2 := by
-  apply eq_smallestMC_of_KC ▸ Modal.instModalCompanion_of_smallestMC_via_KripkeSemantics
-    (IL := Propositional.KC)
-    (IC := Propositional.Kripke.FrameClass.KC)
-    (MC := Modal.Kripke.FrameClass.S4Point2)
-  rintro F hF;
-  simp_all only [Set.mem_setOf_eq];
-  constructor;
+  apply h₂ u Rzu;
+  apply Modal.gödelTranslated_persistency h₁ Ryu;
 
 end S4Point2
 
 
-instance : Propositional.KC.smallestMC ⪯ Modal.GrzPoint2 := calc
-  _ ≊ Modal.S4Point2  := by symm; infer_instance;
-  _ ⪯ Modal.GrzPoint2 := inferInstance
+namespace Propositional.KC
 
+lemma provable_S4Point2_of_mem : φ ∈ Propositional.KC → Modal.S4Point2 ⊢ φᵍ := by
+  apply Propositional.Hilbert.provable_gödelTranslated_of_mem_logic;
+  rintro _ ⟨a, (⟨_, rfl⟩ | ⟨_, rfl⟩), rfl⟩ <;> simp;
 
-namespace GrzPoint2
+theorem modalCompanion_S4Point2 : ModalCompanion Propositional.KC Modal.S4Point2 := by
+  apply modalCompanion_via_kripkeSemantics (P := λ F => IsPiecewiseStronglyConvergent F);
+  . apply provable_S4Point2_of_mem;
+  . intro φ;
+    apply Hilbert.KC.instKripkeComplete.complete;
+  . rintro φ hφ F _ _;
+    apply Modal.instSoundLogicNatFormulaFrameClassS4Point2S4Point2.sound;
+    . grind;
+    . apply Set.mem_setOf_eq.mpr;
+      exact {};
 
-instance : Modal.GrzPoint2 ≊ Propositional.KC.largestMC := by
-  apply Logic.equiv_of_provable;
-  intro φ;
-  constructor;
-  . intro hφ;
-    induction hφ using Modal.Hilbert.Normal.rec! with
-    | axm _ h =>
-      rcases h with (rfl | rfl | rfl);
-      . simp;
-      . simp;
-      . apply WeakerThan.pbl (𝓢 := Propositional.KC.smallestMC); simp;
-    | mdp ihφψ ihψ => exact ihφψ ⨀ ihψ;
-    | nec ihφ => exact nec! ihφ;
-    | _ => apply Logic.sumNormal.mem₁!; simp;
-  . intro hφ;
-    induction hφ using Logic.sumNormal.rec! with
-    | mdp ihφψ ihψ => exact ihφψ ⨀ ihψ;
-    | subst ih => apply Logic.subst _ ih;
-    | nec ih => apply nec! ih;
-    | mem₁ h => apply WeakerThan.pbl h;
-    | mem₂ h => rcases h with ⟨φ, hφ, rfl⟩; simp;
+lemma provable_GrzPoint2_of_mem : φ ∈ Propositional.KC → Modal.GrzPoint2 ⊢ φᵍ := fun h ↦ WeakerThan.pbl $ provable_S4Point2_of_mem h
 
-lemma is_largestMC_of_KC : Modal.GrzPoint2 = Propositional.KC.largestMC := Logic.eq_of_equiv
+theorem modalCompanion_GrzPoint2 : ModalCompanion Propositional.KC Modal.GrzPoint2 := by
+  apply modalCompanion_via_kripkeSemantics (P := λ {κ} F => Finite κ ∧ IsPiecewiseStronglyConvergent F);
+  . apply provable_GrzPoint2_of_mem;
+  . intro φ;
+    apply Hilbert.KC.instKripkeCompleteFinite.complete;
+  . rintro φ hφ F _ ⟨_, _⟩;
+    apply Modal.instSoundLogicNatFormulaFrameClassGrzPoint2Finite_GrzPoint2.sound;
+    . grind;
+    . apply Set.mem_setOf_eq.mpr;
+      exact {};
 
-instance : Sound Propositional.KC.largestMC FrameClass.finite_GrzPoint2 := Kripke.sound_frameClass_of_equiv Modal.GrzPoint2 Propositional.KC.largestMC
+end Propositional.KC
 
-instance : ModalCompanion Propositional.KC Modal.GrzPoint2 := by
-  apply is_largestMC_of_KC ▸ Modal.instModalCompanion_of_largestMC_via_KripkeSemantics
-    Propositional.Kripke.FrameClass.finite_KC
-    FrameClass.finite_GrzPoint2
-  rintro F hF;
-  simp_all only [Set.mem_setOf_eq];
-  exact {}
+end LO
 
-end GrzPoint2
-
-end LO.Modal
 end
