Foundation/Modal/ModalCompanion/Standard/LC.lean
@@ -1,155 +1,76 @@
 module
 
 public import Foundation.Logic.Embedding
-public import Foundation.Modal.ModalCompanion.Standard.Int
-public import Foundation.Modal.Boxdot.GLPoint3_GrzPoint3
--- public import Foundation.Propositional.Kripke.Logic.LC
+public import Foundation.Modal.Boxdot.GL_Grz
+public import Foundation.Modal.Kripke.Logic.GrzPoint3
+public import Foundation.Modal.ModalCompanion.Standard.Basic
+public import Foundation.Propositional.Kripke.Hilbert.LC
 
 @[expose] public section
 
-namespace LO.Modal
+namespace LO
 
 open LO.Entailment LO.Entailment.FiniteContext LO.Modal.Entailment
 open Propositional
-open Propositional.Formula (atom gödelTranslate)
+open Propositional.Formula (gödelTranslate)
 open Propositional.Logic (smallestMC largestMC)
 open Modal
 open Modal.Kripke
-open Modal.Formula.Kripke
 
-@[simp]
-lemma S4.CCLL_CCL : Modal.S4 ⊢ □(□φ 🡒 □ψ) 🡒 □(□φ 🡒 ψ) := by
-  apply Complete.complete (𝓜 := FrameClass.S4);
-  rintro F ⟨_, _⟩ V x h₁ y Rxy h₂;
-  apply @h₁ y Rxy h₂;
-  apply Std.Refl.refl;
-
-instance : Entailment.HasAxiomPoint3 (smallestMC Propositional.LC) where
-  Point3 φ ψ := by
-    constructor;
-    apply Modal.Logic.iff_provable.mp;
-    apply Modal.Logic.subst (L := (smallestMC Propositional.LC)) (φ := Modal.Axioms.Point3 (.atom 0) (.atom 1)) (s := λ a => match a with | 0 => φ | 1 => ψ | _ => .atom a);
-    have : (smallestMC Propositional.LC) ⊢ □(□.atom 0 🡒 □.atom 1) ⋎ □(□.atom 1 🡒 □.atom 0) := by
-      apply Logic.sumNormal.mem₂!;
-      use Axioms.Dummett (.atom 0) (.atom 1);
-      constructor;
-      . apply Propositional.Logic.iff_provable.mp;
-        simp;
-      . tauto;
-    apply ?_ ⨀ this;
-    apply CAA!_of_C!_of_C! <;>
-    . apply Entailment.WeakerThan.pbl (𝓢 := Modal.S4);
-      simp;
 
 namespace S4Point3
 
-lemma gödelTranslated_axiomDummett : Modal.S4Point3 ⊢ □(□ψᵍ 🡒 χᵍ) 🡒 □(ψᵍ 🡒 χᵍ) := by
-  apply axiomK'!;
-  apply nec!;
-  apply C!_swap;
-  apply deduct'!;
-  apply deduct!;
-  have h₁ : [□ψᵍ 🡒 χᵍ, ψᵍ] ⊢[Modal.S4Point3] ψᵍ 🡒 □ψᵍ := of'! $ gödelTranslated_axiomTc;
-  have h₂ : [□ψᵍ 🡒 χᵍ, ψᵍ] ⊢[Modal.S4Point3] ψᵍ := by_axm!;
-  have h₃ : [□ψᵍ 🡒 χᵍ, ψᵍ] ⊢[Modal.S4Point3] □ψᵍ 🡒 χᵍ := by_axm!;
-  exact h₃ ⨀ (h₁ ⨀ h₂);
-
-instance : Modal.S4Point3 ≊ Propositional.LC.smallestMC := by
-  apply Logic.equiv_of_provable;
-  intro φ;
-  constructor;
-  . intro hφ;
-    induction hφ using Modal.Hilbert.Normal.rec! with
-    | axm s h =>
-      rcases h with (rfl | rfl | rfl | rfl) <;> simp;
-    | mdp ihφψ ihφ => exact ihφψ ⨀ ihφ;
-    | nec ihφ => exact nec! ihφ;
-    | _ => simp;
-  . intro hφ;
-    induction hφ using Logic.sumNormal.rec! with
-    | mem₁ h => apply WeakerThan.pbl h;
-    | mdp ihφψ ihψ => exact ihφψ ⨀ ihψ;
-    | nec ihφ => exact nec! ihφ;
-    | subst ihφ => apply Logic.subst _ ihφ;
-    | mem₂ h =>
-      rcases h with ⟨φ, hφ, rfl⟩;
-      apply provable_gödelTranslated_of_provable ?_ (Propositional.Logic.iff_provable.mpr hφ);
-      rintro _ ⟨_, (rfl | rfl), ⟨s, rfl⟩⟩;
-      . simp;
-      . apply A!_replace axiomPoint3! <;>
-        apply S4Point3.gödelTranslated_axiomDummett;
-
-lemma eq_smallestMC_of_KC : Modal.S4Point3 = Propositional.LC.smallestMC := Logic.eq_of_equiv
-
-instance : Sound Propositional.LC.smallestMC FrameClass.S4Point3 := Kripke.sound_frameClass_of_equiv Modal.S4Point3 Propositional.LC.smallestMC
-
-instance : ModalCompanion Propositional.LC Modal.S4Point3 := by
-  apply eq_smallestMC_of_KC ▸ Modal.instModalCompanion_of_smallestMC_via_KripkeSemantics
-    (IL := Propositional.LC)
-    (IC := Propositional.Kripke.FrameClass.LC)
-    (MC := Modal.Kripke.FrameClass.S4Point3)
-  rintro F hF;
-  simp_all only [Set.mem_setOf_eq];
-  constructor;
+@[simp, grind .]
+lemma gödelTranslated_axiomDummett : Modal.S4Point3 ⊢ (Axioms.Dummett φ ψ)ᵍ := by
+  apply Complete.complete (𝓜 := FrameClass.S4Point3);
+  intro F hF V x;
+  replace hF := Set.mem_setOf_eq.mp hF;
+  apply Modal.Formula.Kripke.Satisfies.or_def.mpr;
+  by_contra! hC;
+  rcases hC with ⟨h₁, h₂⟩;
+  obtain ⟨y, Rxy, hy⟩ := Modal.Formula.Kripke.Satisfies.not_box_def.mp h₁;
+  obtain ⟨hyφ, hyψ⟩ := Modal.Formula.Kripke.Satisfies.not_imp_def.mp hy;
+  obtain ⟨z, Rxz, hz⟩ := Modal.Formula.Kripke.Satisfies.not_box_def.mp h₂;
+  obtain ⟨hzφ, hzψ⟩ := Modal.Formula.Kripke.Satisfies.not_imp_def.mp hz;
+  rcases F.ps_connected Rxy Rxz with (Ryz | Rzy);
+  . apply hzψ $ Modal.gödelTranslated_persistency hyφ Ryz;
+  . apply hyψ $ Modal.gödelTranslated_persistency hzφ Rzy;
 
 end S4Point3
 
 
-instance : Propositional.LC.smallestMC ⪯ Modal.GrzPoint3 := calc
-  _ ≊ Modal.S4Point3  := by symm; infer_instance;
-  _ ⪯ Modal.GrzPoint3 := inferInstance
+namespace Propositional.LC
 
+lemma provable_S4Point3_of_mem : φ ∈ Propositional.LC → Modal.S4Point3 ⊢ φᵍ := by
+  apply Propositional.Hilbert.provable_gödelTranslated_of_mem_logic;
+  rintro _ ⟨a, (⟨_, rfl⟩ | ⟨_, _, rfl⟩), rfl⟩ <;> simp;
 
+theorem modalCompanion_S4Point3 : ModalCompanion Propositional.LC Modal.S4Point3 := by
+  apply modalCompanion_via_kripkeSemantics (P := λ F => IsPiecewiseStronglyConnected F);
+  . apply provable_S4Point3_of_mem;
+  . intro φ;
+    apply Hilbert.LC.instKripkeComplete.complete;
+  . rintro φ hφ F _ _;
+    apply Modal.instSoundLogicNatFormulaFrameClassS4Point3S4Point3.sound;
+    . grind;
+    . apply Set.mem_setOf_eq.mpr;
+      exact {};
 
-section GrzPoint3
+lemma provable_GrzPoint3_of_mem : φ ∈ Propositional.LC → Modal.GrzPoint3 ⊢ φᵍ := fun h ↦ WeakerThan.pbl $ provable_S4Point3_of_mem h
 
-instance : Modal.GrzPoint3 ≊ Propositional.LC.largestMC := by
-  apply Logic.equiv_of_provable;
-  intro φ;
-  constructor;
-  . intro hφ;
-    induction hφ using Modal.Hilbert.Normal.rec! with
-    | axm _ h =>
-      rcases h with (rfl | rfl | rfl);
-      . simp;
-      . simp;
-      . apply WeakerThan.pbl (𝓢 := Propositional.LC.smallestMC); simp;
-    | mdp ihφψ ihψ => exact ihφψ ⨀ ihψ;
-    | nec ihφ => exact nec! ihφ;
-    | _ => apply Logic.sumNormal.mem₁!; simp;
-  . intro hφ;
-    induction hφ using Logic.sumNormal.rec! with
-    | mdp ihφψ ihψ => exact ihφψ ⨀ ihψ;
-    | subst ih => apply Logic.subst _ ih;
-    | nec ih => apply nec! ih;
-    | mem₁ h => apply WeakerThan.pbl h;
-    | mem₂ h => rcases h with ⟨φ, hφ, rfl⟩; simp;
+theorem modalCompanion_GrzPoint3 : ModalCompanion Propositional.LC Modal.GrzPoint3 := by
+  apply modalCompanion_via_kripkeSemantics (P := λ {κ} F => Finite κ ∧ IsPiecewiseStronglyConnected F);
+  . apply provable_GrzPoint3_of_mem;
+  . intro φ;
+    apply Hilbert.LC.instKripkeCompleteFinite.complete;
+  . rintro φ hφ F _ ⟨_, _⟩;
+    apply Modal.instSoundLogicNatFormulaSetFrameGrzPoint3SetOfIsFiniteGrzPoint3'.sound;
+    . grind;
+    . apply Set.mem_setOf_eq.mpr;
+      exact {};
 
-lemma is_largestMC_of_LC : Modal.GrzPoint3 = Propositional.LC.largestMC := Logic.eq_of_equiv
+end Propositional.LC
 
-instance : Sound Propositional.LC.largestMC FrameClass.finite_GrzPoint3 := Kripke.sound_frameClass_of_equiv Modal.GrzPoint3 Propositional.LC.largestMC
+end LO
 
-instance : ModalCompanion Propositional.LC Modal.GrzPoint3 := by
-  apply is_largestMC_of_LC ▸ Modal.instModalCompanion_of_largestMC_via_KripkeSemantics
-    Propositional.Kripke.FrameClass.finite_LC
-    ({ F : Frame | F.IsFiniteGrzPoint3' })
-  rintro F hF;
-  simp_all only [Set.mem_setOf_eq];
-  exact {}
-
-end GrzPoint3
-
-
-section boxdot
-
-theorem embedding_LC_GLPoint3 {φ : Propositional.Formula ℕ} : Propositional.LC ⊢ φ ↔ Modal.GLPoint3 ⊢ φᵍᵇ :=
-  Iff.trans ModalCompanion.companion iff_boxdot_GLPoint3_GrzPoint3.symm
-
-instance : Entailment.FaithfullyEmbeddable Propositional.LC Modal.GLPoint3 where
-  prop := ⟨(·ᵍᵇ), fun _ ↦ embedding_LC_GLPoint3.symm⟩
-
-end boxdot
-
-
-end LO.Modal
 end
